\subsubsection{Repeated Quadratic Factors}
\noindent
If a quadratic factor that can't be broken into linear factors is repeated, then we can write
$Q(x) = R(x)(ax^2+bx+c)^k$, $k \geq 0$, and $R(x)$ is not divisible by $(ax^2+bx+c)^k$.
Now we have to do a combination of what we did for repeated linear factors and quadratic factors.
We say
\begin{equation*}
	\frac{P(x)}{R(x)(ax^2+bx+c)^k}=\left(\text{Decomposition of }R(x)\right)+\frac{A_1x+B_1}{ax^2+bx+c}+\ldots+\frac{A_kx+B_k}{(ax^2+bx+c)^k}.
\end{equation*}
We then solve for the coefficients in the numerator.

\begin{example}
	Find the partial fraction decomposition of the following expression:
	\begin{equation*}
		\frac{3x^4-2x^3+6x^2-3x+3}{x^5+3x^4+4x^3+12x^2+4x+12}.
	\end{equation*}
\end{example}
\begin{answer}
	Factoring,
	\begin{equation*}
		x^5+3x^4+4x^3+12x^2+4x+12 = (x+3)(x^2+2)^2.
	\end{equation*}
	So,
	\begin{equation*}
		\frac{3x^4-2x^3+6x^2-3x+3}{x^5+3x^4+4x^3+12x^2+4x+12} = \frac{A_1}{x+3}+\frac{A_2x+B_2}{x^2+2}+\frac{A_3x+B_3}{(x^2+2)^2}.
	\end{equation*}
	Multiplying each side by the denominator,
	\begin{equation*}
		3x^4-2x^3+6x^2-3x+3 = A_1(x^2+2)^2+(A_2x+B_2)(x^2+2)(x+3)+(A_3x+B_3)(x+3).
	\end{equation*}
	At $x=-3$,
	\begin{equation*}
		363 = 121A_1 \implies A_1 = 3.
	\end{equation*}
	Now, we'll use our result for $A_1$ and pick a value for $x$ that minimizes the number of things we need to solve for. We'll have to solve a linear system with 4 unknowns, so we'll need up to 4 values.
	At $x=0$,
	\begin{equation*}
		3 = 3(2)^2 + B_2(2)(3)+B_3(3) \implies 2B_2 + B_3 = -3.
	\end{equation*}
	At $x=1$,
	\begin{equation*}
		7 = 3(3)^2 + (A_2+B_2)(3)(4) + (A_3+B_3)(4) \implies 3A_2 + A_3 + 3B_2 + B_3 = -5.
	\end{equation*}
	At $x=-1$,
	\begin{equation*}
		17 = 3(3)^2 + (-A_2+B_2)(3)(2) + (-A_3+B_3)(2) \implies -3A_2 - A_3 + 3B_2 + B_3 = -5.
	\end{equation*}
	At $x=2$,
	\begin{equation*}
		53 = 3(6)^2 + (2A_2+B_2)(6)(5) + (2A_3+B_3)(5) \implies 12A_2 + 2A_3 + 6B_2 + B_3 = -11.
	\end{equation*}
	Now we have the following system of equations:
	\begin{equation*}
		\begin{cases}
			0A_2  + 0A_3 + 2B_2 + B_3 &= -3 \\
			3A_2  + A_3  + 3B_2 + B_3 &= -5 \\
			-3A_2 - A_3  + 3B_2 + B_3 &= -5 \\
			12A_2 + 2A_3 + 6B_2 + B_3 &= -11
		\end{cases}.
	\end{equation*}
	Solving,
	\begin{equation*}
		A_2 = 0, A_3 = 0, B_2 = -2, \text{ and } B_3 = 1.
	\end{equation*}
	So,
	\begin{equation*}
		\frac{3x^4-2x^3+6x^2-3x+3}{x^5+3x^4+4x^3+12x^2+4x+12} = \frac{3}{x+3}-\frac{2}{x^2+2}+\frac{1}{(x^2+2)^2}.
	\end{equation*}
\end{answer}