\subsection{Test 2}
\begin{enumerate}
	\item Consider the function $f(x,y) = x^2 - 2x + y^2 - 4y + 7$.\\
	\begin{enumerate}[label=\alph*.]
		\item Find equations for an plot (if possible) the C-level curves of $f$ for $C = 3$ and $C = 1$.\\
		We will try to find the level curve for any $C$ and then plug in 1 and 3.
		\begin{align*}
			x^2 - 2x + y^2 - 4y + 7 &= C
			x^2 - 2x + 1 + y^2 - 4y + 4 &= C-2
			(x-1)^2 + (y-2)^2 &= C-2		.
		\end{align*}
		A circle of radius $\sqrt{C-2}$ centered at $(1,2)$.
		For $C = 1$, the level curve does not exist because the circle would have a radius of $\sqrt{2-1} = \sqrt{-1}$.
		For $C = 3$, the level curve is 
		\begin{equation*}
			(x-1)^2 + (y-2)^2 = 1
		\end{equation*}
		
		\begin{figure}[H]
			\centering
			\includegraphics[scale=.25]{./additionalMaterials/test2_circle.png}
		\end{figure}
		
		\item Compute $\nabla f$.
		\begin{equation*}
			\nabla f = \langle f_x, f_y\rangle = \langle 2x-2, 2y-4 \rangle
		\end{equation*}
		
		\item Find the equation of the plane tangent to the surface $z = f(x,y)$ at the point $(x_0, y_0, z_0) = (2,4,7)$.
		\begin{equation*}
			\vec{n} = \langle f_x, f_y, -1\rangle = \langle 2x-2, 2y-4, -1 \rangle.
		\end{equation*}
		At $(2,4,7)$, $\vec{n} = \langle 2, 7, -1 \rangle$. So, the plane equation is 
		\begin{equation*}
			\langle 2, 7, -1 \rangle \cdot \langle x-2, y-4, z-7 \rangle = 0
		\end{equation*}
		
		\item Perform one iteration of gradient descent on $f(x,y)$ with a learning rate $delta = 1/4$ starting from the point $(x_0,y_0) = (2,4)$.\\
		\begin{align*}
			(x_n, y_n) &= (x_{n-1},y_{n-1}) - \delta\nabla f \\
			(x_0, y_0) &= (2,4), \delta = 1/4 \text{, and } \nabla f = \langle 	2x-2, 2y-4 \rangle \\
			(x_1, y_1) &= (2,4) - \frac{1}{4} \langle 2(2)-2, 2(4)-4 \rangle \\
			&= (3/2, 3)
		\end{align*}
	\end{enumerate}

	\item Recall that for a differentiable function $f(x,y)$ and the unit vector $\hat{u} = \langle a, b \rangle$, we proved that $D_{\hat{u}}f = \nabla f \cdot \hat{u}$.
	\begin{enumerate}[label=\alph*.]
		\item Prove the statement ``The gradient is the direction of steepest ascent'' by showing that the directional derivative $D_{\hat{u}}f$ is maximized when $\hat{u}\parallel\nabla f$.
		\begin{equation*}
			D_{\hat{u}}f = \nabla f \cdot \hat{u}=\norm{\nabla f}\norm{\hat{u}}\cos{\theta} = \norm{\nabla f}\cos{\theta}.
		\end{equation*}
		This value is maximized when $\theta$ is a multiple of $2\pi$, meaning that the angle between $\nabla f$ and $\hat{u}$ is 0. This means that the maximum value of the directional derivative, the direction of steepest ascent, is in the same direction as $\nabla f$.\\
			
		\item State the limit definition of the directional derivative $D_{\hat{u}}f$. Starting from that definition, prove that $D_{\hat{u}}f = \nabla f\cdot\hat{u}$.\\
		\begin{align*}
			D_{\hat{u}}f &= \lim_{h \to 0}{\frac{f(x+ah, y+bh)}{h}} \text{ and} \hat{u}=\langle a, b \rangle \\
			&= \lim_{h \to 0}{\frac{f(x+ah, y+bh) - f(x+ah, y)}{h} + \frac{f(x+ah, y) - f(x,y)}{h}} \\
			&= b\lim_{h \to 0}{\frac{f(x, y+bh) - f(x,y)}{bh}} + a\lim_{h \to 0}{\frac{f(x+ah, y) - f(x,y)}{ah}} \\
			&= bf_y + af_x = \langle f_x, f_y \rangle \cdot \langle a, b \rangle = \nabla f \cdot \hat{u}
		\end{align*}
	\end{enumerate}
	
	\item Use the method of Lagrange Multipliers to find the maximum of the product of two numbers $x$ and $y$ given that $(x,y)$ is a coordinate pair in the 1st quadrant located on the unit circle centered at the origin. Begin by stating the objective function $f(x,y)$ and the constraint equation $g(x,y) = k$.\\
	\begin{itemize}
		\item Objective Function: $f(x,y) = xy$
		\item Constraint Equation: $g(x,y) = x^2 + y^2 = 1$, $x \geq 0$ and $y \geq 0$
	\end{itemize}
	\begin{equation*}
		F(x,y,\lambda) = xy + \lambda(1-x^2-y^2)
	\end{equation*}
	\begin{equation*}
		\frac{\partial F}{\partial x} = y-2\lambda x, \frac{\partial F}{\partial y} = x-2\lambda y \text{ and } \frac{\partial F}{\partial\lambda} = 1-x^2-y^2
	\end{equation*}
	\begin{equation*}
		\langle y-2\lambda x, x-2 \lambda y, 1-x^2-y^2 \rangle = \vec{0}
	\end{equation*}
	\begin{equation*}
		\begin{cases}
			y = 2\lambda x \\
			x = 2\lambda y \\
			x^2 + y^2 = 1
		\end{cases} \implies \begin{cases}
			\lambda = 1/2 \\
			x = 1/\sqrt{2} \\
			y = 1/\sqrt{2}
		\end{cases}.
	\end{equation*}
	So, the maximum product is $\frac{1}{\sqrt{2}} \cdot \frac{1}{\sqrt{2}} = \frac{1}{2}$ at $\left(\frac{1}{\sqrt{2}}, \frac{1}{\sqrt{2}}\right)$\\
	
	\item The function $p(x,y) = \frac{1}{\pi}\exp{\left(-(x-a)^2 - (y-b)^2\right)}$ is the probability density function of a bivariate normal distribution with mean $(a,b)$ and standard deviation $\frac{1}{\sqrt{2}}$. Show that the global maximum of $p(x,y)$ occurs at $(a,b)$.
	\begin{align*}
		p_x &= \frac{1}{\pi}(-2(x-a))\exp{(-((x-a)^2 + (y-b)^2))} \\
		p_y &= \frac{1}{\pi}(-2(y-b))\exp{(-((x-a)^2 + (y-b)^2))}
	\end{align*}
	$p_x = 0$ when $x=a$ and $p_y = 0$ when $y=b$
	$\implies (a,b)$ is a critical point.
	\begin{align*}
		p_{xx} &= \frac{1}{\pi}(-2(y-b))\exp{(-((x-a)^2 + (y-b)^2))} - 2\exp{(-((x-a)^2 + (y-b)^2))} \\
		&= \frac{1}{\pi}(4(x-a)^2 - 2)\exp{(-((x-a)^2 + (y-b)^2))} \\
		p_{yy} &= \frac{1}{\pi}(4(y-b)^2 - 2)\exp{(-((x-a)^2 + (y-b)^2))} \\
		p_{xy} &= p_{yx} = \frac{4}{\pi}(x-a)(y-b)\exp{(-((x-a)^2 + (y-b)^2))} \\
		p_{xx}(a,b) &= \frac{-2}{\pi}, p_{yy}(a,b) = \frac{-2}{\pi} \text{ and } p_{xy}(a,b) = p_{yx}(a,b) = 0
	\end{align*}
	\begin{equation*}
		H(a,b) = \begin{bmatrix}
		\frac{-2}{\pi} & 0 \\
		0 & \frac{-2}{\pi}
		\end{bmatrix}
	\end{equation*}
	\begin{equation*}
		\det{(H(a,b))} = \frac{4}{\pi^2}
	\end{equation*}
	$(a,b)$ is an extrema because $\det{(H(a,b))} > 0$.
	Since $f_{xx}(a,b) < 0$ and $f_{yy}(a,b) < 0$, $(a,b)$ is a maximum.
	$(a,b)$ is a global maximum because $p(x,y)$ is strictly decreasing as you move away from $(a,b)$.\\
	
	\item Let the C-level curve of the function $f(x,y)$ be parameterized by the VVF $\vec{r}(t) = \langle x(t), y(t) \rangle$. Use the chain rule to show that $\nabla f(\vec{r}(t))\perp\vec{r^\prime}(t)$ for all $t$.\\
	Since $\vec{r}(t)$ parameterizes a C-level curve of $f$,
	\begin{equation*}
		f\circ\vec{r}(t) = C.
	\end{equation*}
	Where $C$ is a constant.
	\begin{equation*}
		\frac{\mathrm{d}}{\mathrm{d}t}(f\circ\vec{r}(t)) = \frac{\mathrm{d}}{\mathrm{d}t}C
	\end{equation*}
	\begin{equation*}
		\frac{\partial f}{\partial x}\frac{\mathrm{d}x}{\mathrm{d}t} + \frac{\partial f}{\partial y}\frac{\mathrm{d}y}{\mathrm{d}t} = 0
	\end{equation*}
	\begin{equation*}
		\left<\frac{\partial f}{\partial x}, \frac{\partial f}{\partial y}\right> \cdot \left<\frac{\mathrm{d}x}{\mathrm{d}t}, \frac{\mathrm{d}y}{\mathrm{d}t}\right> = 0
	\end{equation*}
	\begin{align*}
		\nabla f(\vec{r}(t)) &\cdot \vec{r^\prime}(t) = 0 \\
		&\implies \nabla f(\vec{r}(t))\perp\vec{r^\prime}(t)
	\end{align*}
\end{enumerate}